Update PFtoIRThread

src/pf2ir/PFtoIRThread.v
@@ -16,7 +16,6 @@ Require Import Time.
 Require Import View.
 Require Import BoolMap.
 Require Import Promises.
-Require Import Reserves.
 Require Import Cell.
 Require Import Memory.
 Require Import TView.
@@ -36,139 +35,363 @@ Module PFtoIRThread.
   Section PFtoIRThread.
     Variable lang: language.
 
+    Variant sim_memory (mem_pf mem_ir: Memory.t): Prop :=
+      | sim_memory_intro
+          (SOUND: Memory.le mem_pf mem_ir)
+          (COMPLETE: Memory.messages_le mem_ir mem_pf)
+          (GRESERVES: forall loc from to msg
+                        (GET: Memory.get loc to mem_pf = Some (from, msg)),
+              msg <> Message.reserve)
+    .
+    #[local] Hint Constructors sim_memory: core.
+
     Variant sim_thread (th_pf th_ir: Thread.t lang): Prop :=
       | sim_thread_intro
           (STATE: Thread.state th_pf = Thread.state th_ir)
           (TVIEW: Local.tview (Thread.local th_pf) = Local.tview (Thread.local th_ir))
           (PROMISES: Local.promises (Thread.local th_pf) = BoolMap.bot)
-          (RESERVES: Local.reserves (Thread.local th_pf) = BoolMap.bot)
+          (RESERVES: Local.reserves (Thread.local th_pf) = Memory.bot)
           (SC: Global.sc (Thread.global th_pf) = Global.sc (Thread.global th_ir))
           (GPROMISES: Global.promises (Thread.global th_pf) = BoolMap.bot)
-          (GRESERVES: Global.reserves (Thread.global th_pf) = BoolMap.bot)
-          (MEMORY: Global.memory (Thread.global th_pf) = Global.memory (Thread.global th_ir))
+          (MEMORY: sim_memory (Global.memory (Thread.global th_pf)) (Global.memory (Thread.global th_ir)))
     .
     #[local] Hint Constructors sim_thread: core.
 
-    Lemma sim_thread_fully_reserved
+    Lemma sim_memory_cap
+          mem_pf mem_ir
+          (SIM: sim_memory mem_pf mem_ir):
+      sim_memory mem_pf (Memory.cap_of mem_ir).
+    Proof.
+      specialize (Memory.cap_of_cap mem_ir). i.
+      inv SIM. econs; ii; eauto.
+      - inv H. eauto.
+      - exploit Memory.cap_inv; eauto. i. des; ss. eauto.
+      - eapply GRESERVES; eauto.
+    Qed.
+
+    Lemma sim_thread_cap
           th_pf th_ir
           (SIM: PFtoIRThread.sim_thread th_pf th_ir):
-      PFtoIRThread.sim_thread th_pf (Thread.fully_reserved th_ir).
+      PFtoIRThread.sim_thread th_pf (Thread.cap_of th_ir).
     Proof.
       inv SIM. econs; ss.
+      eapply sim_memory_cap; eauto.
+    Qed.
+
+    Lemma sim_memory_add
+          mem1_pf mem1_ir
+          loc from to msg mem2_ir
+          (MEM1: sim_memory mem1_pf mem1_ir)
+          (ADD_IR: Memory.add mem1_ir loc from to msg mem2_ir)
+          (MSG: msg <> Message.reserve):
+      exists mem2_pf,
+        (<<ADD_PF: Memory.add mem1_pf loc from to msg mem2_pf>>) /\
+        (<<MEM2: sim_memory mem2_pf mem2_ir>>).
+    Proof.
+      inv MEM1.
+      exploit (@Memory.add_exists mem1_pf loc from to msg); i.
+      { exploit SOUND; eauto. i.
+        exploit Memory.add_get1; eauto. i.
+        exploit Memory.add_get0; eauto. i. des.
+        exploit Memory.get_disjoint; [exact x1|exact GET0|].
+        i. des; subst; try congr.
+        symmetry. ss.
+      }
+      { inv ADD_IR. inv ADD. ss. }
+      { inv ADD_IR. inv ADD. ss. }
+      des. esplits; eauto. econs; ii.
+      - erewrite Memory.add_o; eauto.
+        revert LHS. erewrite Memory.add_o; try exact x0.
+        condtac; ss; eauto.
+      - erewrite Memory.add_o; eauto.
+        revert LHS. erewrite Memory.add_o; try exact ADD_IR.
+        condtac; ss; eauto.
+      - subst. revert GET.
+        erewrite Memory.add_o; eauto. condtac; ss; i.
+        + des. inv GET. ss.
+        + eapply GRESERVES; eauto.
+    Qed.
+
+    Lemma sim_memory_reserve
+          mem1_pf
+          rsv1_ir mem1_ir
+          loc from to rsv2_ir mem2_ir
+          (MEM1: sim_memory mem1_pf mem1_ir)
+          (RESERVE_IR: Memory.reserve rsv1_ir mem1_ir loc from to rsv2_ir mem2_ir):
+      (<<MEM2: sim_memory mem1_pf mem2_ir>>).
+    Proof.
+      inv MEM1. inv RESERVE_IR. econs; ii.
+      - erewrite Memory.add_o; eauto.
+        condtac; ss; eauto. des. subst.
+        exploit SOUND; eauto. i.
+        exploit Memory.add_get0; try exact MEM. i. des. congr.
+      - revert LHS. erewrite Memory.add_o; eauto.
+        condtac; ss; eauto.
+      - eapply GRESERVES; eauto.
+    Qed.
+
+    Lemma sim_memory_cancel
+          mem1_pf
+          rsv1_ir mem1_ir
+          loc from to rsv2_ir mem2_ir
+          (MEM1: sim_memory mem1_pf mem1_ir)
+          (CANCEL_IR: Memory.cancel rsv1_ir mem1_ir loc from to rsv2_ir mem2_ir):
+      (<<MEM2: sim_memory mem1_pf mem2_ir>>).
+    Proof.
+      inv MEM1. inv CANCEL_IR. econs; ii.
+      - erewrite Memory.remove_o; eauto.
+        condtac; ss; eauto. des. subst.
+        exploit SOUND; eauto. i.
+        exploit Memory.remove_get0; try exact MEM. i. des.
+        rewrite GET in *. inv x0.
+        exploit GRESERVES; eauto. ss.
+      - revert LHS. erewrite Memory.remove_o; eauto.
+        condtac; ss; eauto.
+      - eapply GRESERVES; eauto.
+    Qed.
+
+    Lemma sim_is_racy
+          lc_src gl_src lc_tgt gl_tgt
+          loc to ord
+          (TVIEW: Local.tview lc_src = Local.tview lc_tgt)
+          (MEMORY: sim_memory (Global.memory gl_src) (Global.memory gl_tgt))
+          (RACE_TGT: Local.is_racy lc_tgt gl_tgt loc (Some to) ord):
+      Local.is_racy lc_src gl_src loc (Some to) ord.
+    Proof.
+      inv RACE_TGT.
+      inv MEMORY. exploit COMPLETE; eauto. i.
+      econs 2; eauto. congr.
     Qed.
 
     Lemma sim_thread_internal_step
           th1_pf th1_ir
-          reserved e th2_ir
+          e th2_ir
           (SIM1: sim_thread th1_pf th1_ir)
-          (STEP: Thread.step reserved false e th1_ir th2_ir):
+          (STEP: Thread.step e th1_ir th2_ir)
+          (EVENT: ThreadEvent.is_internal e):
       <<SIM2: sim_thread th1_pf th2_ir>>.
     Proof.
-      inv SIM1. inv STEP. inv LOCAL; inv LOCAL0; ss.
+      inv SIM1. inv STEP; inv LOCAL; ss; inv LOCAL0; ss.
+      - exploit sim_memory_reserve; eauto.
+      - exploit sim_memory_cancel; eauto.
     Qed.
 
-    Lemma sim_thread_program_step
-          th1_pf th1_ir
-          reserved e th2_ir
-          (SIM1: sim_thread th1_pf th1_ir)
-          (STEP: Thread.step reserved true e th1_ir th2_ir)
-          (PF: ~ ThreadEvent.is_racy_promise e):
-      exists th2_pf,
-        (<<STEP_PF: Thread.step TimeMap.bot true e th1_pf th2_pf>>) /\
-        (<<SIM2: sim_thread th2_pf th2_ir>>).
-    Proof.
-      destruct th1_ir as [st1_ir [tview1_ir prm1_ir rsv1_ir] [sc1_ir gprm1_ir grsv1_ir mem1_ir]],
-          th1_pf as [st1_pf [tview1_pf prm1_pf rsv1_pf] [sc1_pf gprm1_pf grsv1_pf mem1_pf]].
-      inv SIM1. ss. subst.
-      inv STEP. inv LOCAL; ss.
-      - esplits; [econs; [|econs 1]|]; eauto.
-      - inv LOCAL0. ss.
-        esplits; [econs; [|econs 2]|]; eauto.
-      - inv LOCAL0. ss.
-        esplits; [econs; [|econs 3]|]; eauto.
-        + econs; ss; try by intuition. eauto.
-        + ss.
-      - inv LOCAL1. inv LOCAL2. ss.
-        esplits; [econs; [|econs 4]|]; eauto.
-        + econs; ss; try by intuition. eauto.
-        + ss.
-      - inv LOCAL0.
-        esplits; [econs; [|econs 5]|]; eauto.
-      - inv LOCAL0.
-        esplits; [econs; [|econs 6]|]; eauto.
-      - esplits; [econs; [|econs 7]|]; eauto.
-      - destruct to; ss. inv LOCAL0. inv RACE. ss.
-        esplits; [econs; [|econs 8]|]; eauto.
-      - destruct to; ss. inv LOCAL0. inv RACE. ss.
-        esplits; [econs; [|econs 9]|]; eauto.
-      - destruct to; ss.
-        + inv LOCAL0. inv RACE. ss.
-          esplits; [econs; [|econs 10]|]; eauto.
-        + esplits; [econs; [|econs 10]|]; eauto.
-          apply not_and_or in PF. des.
-          * econs 1. destruct ordr; ss.
-          * econs 2. destruct ordw; ss.
-    Qed.
+    (* Lemma sim_thread_program_step *)
+    (*       th1_pf th1_ir *)
+    (*       reserved e th2_ir *)
+    (*       (SIM1: sim_thread th1_pf th1_ir) *)
+    (*       (STEP: Thread.step reserved true e th1_ir th2_ir) *)
+    (*       (PF: ~ ThreadEvent.is_racy_promise e): *)
+    (*   exists th2_pf, *)
+    (*     (<<STEP_PF: Thread.step TimeMap.bot true e th1_pf th2_pf>>) /\ *)
+    (*     (<<SIM2: sim_thread th2_pf th2_ir>>). *)
+    (* Proof. *)
+    (*   destruct th1_ir as [st1_ir [tview1_ir prm1_ir rsv1_ir] [sc1_ir gprm1_ir grsv1_ir mem1_ir]], *)
+    (*       th1_pf as [st1_pf [tview1_pf prm1_pf rsv1_pf] [sc1_pf gprm1_pf grsv1_pf mem1_pf]]. *)
+    (*   inv SIM1. ss. subst. *)
+    (*   inv STEP. inv LOCAL; ss. *)
+    (*   - esplits; [econs; [|econs 1]|]; eauto. *)
+    (*   - inv LOCAL0. ss. *)
+    (*     esplits; [econs; [|econs 2]|]; eauto. *)
+    (*   - inv LOCAL0. ss. *)
+    (*     esplits; [econs; [|econs 3]|]; eauto. *)
+    (*     + econs; ss; try by intuition. eauto. *)
+    (*     + ss. *)
+    (*   - inv LOCAL1. inv LOCAL2. ss. *)
+    (*     esplits; [econs; [|econs 4]|]; eauto. *)
+    (*     + econs; ss; try by intuition. eauto. *)
+    (*     + ss. *)
+    (*   - inv LOCAL0. *)
+    (*     esplits; [econs; [|econs 5]|]; eauto. *)
+    (*   - inv LOCAL0. *)
+    (*     esplits; [econs; [|econs 6]|]; eauto. *)
+    (*   - esplits; [econs; [|econs 7]|]; eauto. *)
+    (*   - destruct to; ss. inv LOCAL0. inv RACE. ss. *)
+    (*     esplits; [econs; [|econs 8]|]; eauto. *)
+    (*   - destruct to; ss. inv LOCAL0. inv RACE. ss. *)
+    (*     esplits; [econs; [|econs 9]|]; eauto. *)
+    (*   - destruct to; ss. *)
+    (*     + inv LOCAL0. inv RACE. ss. *)
+    (*       esplits; [econs; [|econs 10]|]; eauto. *)
+    (*     + esplits; [econs; [|econs 10]|]; eauto. *)
+    (*       apply not_and_or in PF. des. *)
+    (*       * econs 1. destruct ordr; ss. *)
+    (*       * econs 2. destruct ordw; ss. *)
+    (* Qed. *)
 
     Lemma sim_thread_step
           th1_pf th1_ir
-          reserved pf e_ir th2_ir
+          e_ir th2_ir
           (SIM1: sim_thread th1_pf th1_ir)
-          (STEP: Thread.step reserved pf e_ir th1_ir th2_ir)
+          (STEP: Thread.step e_ir th1_ir th2_ir)
           (PF: ~ ThreadEvent.is_racy_promise e_ir):
       exists e_pf th2_pf,
-        (<<STEP_PF: Thread.opt_step TimeMap.bot true e_pf th1_pf th2_pf>>) /\
+        (<<STEP_PF: Thread.opt_step e_pf th1_pf th2_pf>>) /\
+        (<<EVENT_PF: ThreadEvent.is_program e_pf>>) /\
         (<<EVENT: __guard__ (
-                      ThreadEvent.get_machine_event_pf e_pf <> MachineEvent.failure /\
-                      ThreadEvent.get_machine_event_pf e_pf = ThreadEvent.get_machine_event e_ir \/
-                      ThreadEvent.get_machine_event_pf e_pf = MachineEvent.failure)>>) /\
+                      e_pf = ThreadEvent.silent /\ ThreadEvent.is_internal e_ir \/
+                      e_pf = e_ir)>>) /\
         (<<SIM2: sim_thread th2_pf th2_ir>>).
     Proof.
-      destruct pf.
-      - exploit sim_thread_program_step; eauto. i. des.
-        esplits; [econs 2|..]; eauto. unguard.
-        destruct e_ir; ss; auto; left; split; ss.
-      - exploit sim_thread_internal_step; eauto. i. des.
-        esplits; [econs 1|..]; eauto. unguard.
-        inv STEP. inv LOCAL; ss; left; split; ss.
+      unguard.
+      destruct th1_ir as [st1_ir [tview1_ir prm1_ir rsv1_ir] [sc1_ir gprm1_ir mem1_ir]],
+          th1_pf as [st1_pf [tview1_pf prm1_pf rsv1_pf] [sc1_pf gprm1_pf mem1_pf]].
+      inv SIM1. ss. subst.
+      inv STEP; inv LOCAL; ss.
+      { (* promise *)
+        inv LOCAL0. ss.
+        esplits; [econs 1|..]; eauto; ss.
+      }
+      { (* reserve *)
+        inv LOCAL0. ss.
+        exploit sim_memory_reserve; try exact RESERVE; eauto. i. des.
+        esplits; [econs 1|..]; eauto; ss.
+      }
+      { (* cancel *)
+        inv LOCAL0. ss.
+        exploit sim_memory_cancel; try exact RESERVE; eauto. i. des.
+        esplits; [econs 1|..]; eauto; ss.
+      }
+      { (* silent *)
+        esplits.
+        - econs 2. econs 2; [|econs 1]; eauto.
+        - ss.
+        - right. ss.
+        - ss.
+      }
+      { (* read *)
+        inv LOCAL0. ss.
+        dup MEMORY. inv MEMORY0. exploit COMPLETE; eauto. i.
+        esplits.
+        - econs 2. econs 2; [|econs 2]; eauto.
+        - ss.
+        - right. ss.
+        - ss.
+      }
+      { (* write *)
+        inv LOCAL0. ss.
+        exploit sim_memory_add; try exact WRITE; eauto; ss. i. des.
+        esplits.
+        - econs 2. econs 2; [|econs 3]; eauto.
+        - ss.
+        - right. ss.
+        - ss.
+      }
+      { (* update *)
+        inv LOCAL1. inv LOCAL2. ss.
+        dup MEMORY. inv MEMORY0. exploit COMPLETE; eauto. i.
+        exploit sim_memory_add; try exact WRITE; eauto; ss. i. des.
+        esplits.
+        - econs 2. econs 2; [|econs 4]; eauto.
+        - ss.
+        - right. ss.
+        - ss.
+      }
+      { (* fence *)
+        inv LOCAL0. ss.
+        esplits.
+        - econs 2. econs 2; [|econs 5]; eauto.
+        - ss.
+        - right. ss.
+        - ss.
+      }
+      { (* syscall *)
+        inv LOCAL0. ss.
+        esplits.
+        - econs 2. econs 2; [|econs 6]; eauto.
+        - ss.
+        - right. ss.
+        - ss.
+      }
+      { (* failure *)
+        inv LOCAL0. ss.
+        esplits.
+        - econs 2. econs 2; [|econs 7]; eauto.
+        - ss.
+        - right. ss.
+        - ss.
+      }
+      { (* racy read *)
+        inv LOCAL0. destruct to; ss.
+        esplits.
+        - econs 2. econs 2; [|econs 8]; eauto.
+          econs. eapply sim_is_racy; try eapply RACE; ss.
+        - ss.
+        - right. ss.
+        - ss.
+      }
+      { (* racy write *)
+        inv LOCAL0. destruct to; ss.
+        esplits.
+        - econs 2. econs 2; [|econs 9]; eauto.
+          econs. eapply sim_is_racy; try eapply RACE; ss.
+        - ss.
+        - right. ss.
+        - ss.
+      }
+      { (* racy update *)
+        destruct to; ss.
+        - esplits.
+          + econs 2. econs 2; [|econs 10]; eauto.
+            inv LOCAL0. econs 3.
+            eapply sim_is_racy; try eapply RACE; ss.
+          + ss.
+          + right. ss.
+          + ss.
+        - esplits.
+          + econs 2. econs 2; [|econs 10]; eauto.
+            apply not_and_or in PF. des.
+            * econs 1; ss. destruct ordr; ss.
+            * econs 2; ss. destruct ordw; ss.
+          + ss.
+          + right. ss.
+          + ss.
+      }
     Qed.
 
     Lemma rtc_tau_step_cases
-          reserved th1 th2
-          (STEPS: rtc (@Thread.tau_step lang reserved) th1 th2):
-      (<<STEPS: rtc (pstep (Thread.step_allpf reserved) (strict_pf /1\ ThreadEvent.is_silent)) th1 th2>>) \/
-      exists th pf e th2,
-        (<<STEPS: rtc (pstep (Thread.step_allpf reserved) (strict_pf /1\ ThreadEvent.is_silent)) th1 th>>) /\
-        (<<STEP_RACE: Thread.step reserved pf e th th2>>) /\
+          th1 th2
+          (STEPS: rtc (@Thread.tau_step lang) th1 th2):
+      (<<STEPS: rtc (pstep (@Thread.step _)
+                           (fun e => ~ ThreadEvent.is_racy_promise e /\ ThreadEvent.is_silent e))
+                    th1 th2>>) \/
+      exists th e th2,
+        (<<STEPS: rtc (pstep (@Thread.step _)
+                             (fun e => ~ ThreadEvent.is_racy_promise e /\ ThreadEvent.is_silent e))
+                      th1 th>>) /\
+        (<<STEP_RACE: Thread.step e th th2>>) /\
         (<<EVENT_RACE: ThreadEvent.is_racy_promise e>>).
     Proof.
-      induction STEPS; eauto.
-      inv H. inv TSTEP.
-      destruct (classic (strict_pf e)).
+      induction STEPS; eauto. inv H.
+      destruct (classic (ThreadEvent.is_racy_promise e)).
+      - right. esplits; try exact STEP; eauto.
       - des.
         + left. econs 2; eauto.
         + right. esplits; try exact STEP_RACE; eauto.
-      - right. esplits; try exact STEP; eauto.
-        apply NNPP in H. ss.
     Qed.
 
     Lemma sim_thread_rtc_step
           th1_pf th1_ir
-          reserved th2_ir
+          th2_ir
           (SIM1: sim_thread th1_pf th1_ir)
-          (STEPS: rtc (pstep (Thread.step_allpf reserved) (strict_pf /1\ ThreadEvent.is_silent)) th1_ir th2_ir):
+          (STEPS: rtc (pstep (@Thread.step _)
+                             (fun e => ~ ThreadEvent.is_racy_promise e /\ ThreadEvent.is_silent e))
+                      th1_ir th2_ir):
       exists th2_pf,
-        (<<STEPS_PF: rtc (tau (Thread.step TimeMap.bot true)) th1_pf th2_pf>>) /\
+        (<<STEPS_PF: rtc (pstep (@Thread.step _)
+                                (fun e => ThreadEvent.is_program e /\ ThreadEvent.is_silent e))
+                         th1_pf th2_pf>>) /\
         (<<SIM2: sim_thread th2_pf th2_ir>>).
     Proof.
       revert th1_pf SIM1.
       induction STEPS; i; eauto.
-      inv H. inv STEP. des.
-      destruct pf.
-      - exploit sim_thread_program_step; eauto. i. des.
-        exploit IHSTEPS; eauto. i. des.
-        esplits; [econs 2|]; eauto.
-      - exploit sim_thread_internal_step; eauto.
+      inv H. des.
+      exploit sim_thread_step; eauto. i. des.
+      exploit IHSTEPS; eauto. i. des.
+      inv STEP_PF; eauto.
+      esplits; try exact SIM0.
+      econs 2; eauto. econs; eauto. split; ss.
+      unguard. des; subst; ss.
     Qed.
   End PFtoIRThread.
 End PFtoIRThread.
